Finish proof

code/mlkem/Hacl.MLkem.Poly.fst
@@ -43,6 +43,24 @@ let add_zq a b =
   // assert (v sub_value == 0 \/ v sub_value == v q ) ;
   sum -. sub_value
 
+let empty #a: lseq a 0 = FStar.Seq.empty
+
+let cons #a #len (elem:a) (s:lseq a len): lseq a (len + 1) = FStar.Seq.cons elem s
+
+val slice_plus_one (#a:Type) (#len1 #len2:size_nat) (s1: lseq a len1) (s2: lseq a len2) (i: size_nat):
+  Lemma (requires (
+    i < len1 /\
+    i < len2 /\
+    Seq.equal (Seq.slice #_ #len1 s1 0 i) (Seq.slice #_ #len2 s2 0 i) /\
+    Seq.index #_ #len1 s1 i == Seq.index #_ #len2 s2 i))
+  (ensures Seq.equal (Seq.slice #_ #len1 s1 0 (i + 1)) (Seq.slice #_ #len2 s2 0 (i + 1)))
+let slice_plus_one #a #len1 #len2 s1 s2 i =
+  let x = Seq.index #_ #len1 s1 i in
+  let s1' = Seq.concat #_ #i #1 (Seq.slice #_ #len1 s1 0 i) (cons x empty) in
+  let s2' = Seq.concat #_ #i #1 (Seq.slice #_ #len2 s2 0 i) (cons x empty) in
+  assert (Seq.equal s1' (Seq.slice #_ #len1 s1 0 (i + 1)));
+  assert (Seq.equal s2' (Seq.slice #_ #len2 s2 0 (i + 1)))
+
 val add:
     #deg: size_t
   -> a:lpoly deg
@@ -84,7 +102,9 @@ let add #deg a b res =
       let sum = add_zq ai bi in
       res.(i) <- sum;
       let h1 = ST.get () in
-      assume (Seq.equal (Seq.slice (lpoly_v h1 res) 0 (v i + 1)) (Seq.slice spec_sum 0 (v i + 1)))
+      assert (Seq.equal (Seq.slice (lpoly_v h1 res) 0 (v i)) (Seq.slice spec_sum 0 (v i)));
+      assert (Seq.index (lpoly_v h1 res) (v i) == Seq.index spec_sum (v i));
+      slice_plus_one #_ #(v deg) #(v deg) (lpoly_v h1 res) spec_sum (v i)
     in
   Lib.Loops.for 0ul deg inv body;
   pop_frame ()
